Finished kstar section. Regex is WIP

Cslib/Computability/Languages/KleeneAlgorithm.lean
@@ -8,8 +8,8 @@ module
 
 public import Cslib.Computability.Automata.Acceptors.Acceptor
 public import Cslib.Computability.Automata.DA.Basic
+public import Mathlib.Computability.Language
 public import Mathlib.Computability.RegularExpressions
-
 
 /-!
 # Kleene's Algorithm
@@ -88,11 +88,9 @@ theorem language_bddpath_eq_dfa {n k : ℕ} (flts : FLTS (Fin n) Symbol) (i j : 
   simp only [mem_language, Accepts]
   grind
 
-section splitLast
-
 open List
 
--- variable [DecidableEq Symbol]
+section splitLast
 
 /-- The function `splitLastCompl` sends a string to its longest prefix ending at state `t`.
 If the string ends at state `t`, then `splitLastCompl` returns the original string.
@@ -334,8 +332,128 @@ end splitLast
 
 section splitFirst
 
+/-- The function `splitFirst` sends a string to its shortest prefix ending at state `t`.
+The string is empty if and only if its `splitFirst` is empty.
+If the string never passes through state `t` (starting state can be `t`),
+then `splitFirst` returns the original string. -/
+def splitFirst {n : ℕ} (flts : FLTS (Fin n) Symbol) (s t : Fin n) : List Symbol → List Symbol
+  | [] => []
+  | a :: x => if flts.tr s a = t then [a] else a :: splitFirst flts (flts.tr s a) t x
+
+lemma isPrefix_splitFirst {n : ℕ} (flts : FLTS (Fin n) Symbol) (s t : Fin n) (xs : List Symbol) :
+    IsPrefix (splitFirst flts s t xs) xs := by
+  induction xs generalizing s with
+  | nil => simp [splitFirst]
+  | cons a xs ih => grind [splitFirst]
+
+noncomputable def splitFirstCompl {n : ℕ} (flts : FLTS (Fin n) Symbol) (s t : Fin n)
+    (xs : List Symbol) : List Symbol := (isPrefix_splitFirst flts s t xs).choose
+
+lemma splitFirst_append {n : ℕ} (flts : FLTS (Fin n) Symbol) (s t : Fin n) (xs : List Symbol) :
+    splitFirst flts s t xs ++ splitFirstCompl flts s t xs = xs := by
+  grind [splitFirst, splitFirstCompl]
+
+lemma splitFirst_mem {n : ℕ} {flts : FLTS (Fin n) Symbol} {i k : Fin n} {xs : List Symbol}
+    (h : xs ∈ (language (BddPath.mk flts i k (k.val + 1)))) :
+    splitFirst flts i k xs ∈ language (BddPath.mk flts i k k.val) := by
+  induction xs generalizing i with
+  | nil => simpa [Accepts, splitFirst, PathSupp] using h
+  | cons a xs ih =>
+  simp only [mem_language, Accepts, Order.lt_add_one_iff, splitFirst] at ih h ⊢
+  obtain ⟨h1, h2⟩ := h
+  split_ifs with ha
+  · refine ⟨by grind, ?_⟩
+    have : PathSupp flts i [a] = ∅ := by grind [PathSupp]
+    simp [this]
+  · have : flts.mtr i (a :: splitFirst flts (flts.tr i a) k xs) =
+      flts.mtr (flts.tr i a) (splitFirst flts (flts.tr i a) k xs) := by grind
+    by_cases hxs : xs = []
+    · grind
+    rw [pathSupp_head hxs] at h2
+    by_cases hPath : splitFirst flts (flts.tr i a) k xs = []
+    · grind
+    rw [this, pathSupp_head hPath]
+    grind
+
+lemma splitFirst_mem' {n : ℕ} {flts : FLTS (Fin n) Symbol} {i k : Fin n} {xs : List Symbol}
+    (hxs : xs ≠ []) (h : xs ∈ (language (BddPath.mk flts i k (k.val + 1)))) :
+    splitFirst flts i k xs ∈ language (BddPath.mk flts i k k.val) - 1 := by
+  rw [Language.mem_sub]
+  refine ⟨splitFirst_mem h, ?_⟩
+  simp only [Language.mem_one]
+  induction xs with
+  | nil => contradiction
+  | cons a xs ih => grind [splitFirst]
+
+lemma splitFirstCompl_mem {n : ℕ} {flts : FLTS (Fin n) Symbol} {i k : Fin n} {xs : List Symbol}
+    (h : xs ∈ (language (BddPath.mk flts i k (k.val + 1)))) :
+    splitFirstCompl flts i k xs ∈ language (BddPath.mk flts k k (k.val + 1)) := by
+  have h' := splitFirst_mem h
+  simp only [mem_language, Accepts] at h h' ⊢
+  rw [← splitFirst_append flts i k xs] at h
+  refine ⟨by grind, ?_⟩
+  by_cases splitFirst flts i k xs = [] ∨ splitFirstCompl flts i k xs = []
+  · grind [PathSupp]
+  grind [pathSupp_append]
+
+-- The original path2
+lemma language_bddpath_splitFirst {n : ℕ} (flts : FLTS (Fin n) Symbol) (i k : Fin n) :
+    language (BddPath.mk flts i k (k + 1)) =
+    language (BddPath.mk flts i k k) * language (BddPath.mk flts k k (k + 1)) := by
+  ext xs
+  rw [Language.mem_mul]
+  constructor
+  · intro h
+    use splitFirst flts i k xs, splitFirst_mem h,
+      splitFirstCompl flts i k xs, splitFirstCompl_mem h,
+      splitFirst_append flts _ _ _
+  · intro ⟨ys, ⟨⟨hys, hsuppys⟩, ⟨zs, ⟨⟨hzs, hsuppzs⟩, happend⟩⟩⟩⟩
+    refine ⟨by grind, ?_⟩
+    by_cases ys = [] ∨ zs = []
+    · grind
+    grind [pathSupp_append]
+
 end splitFirst
 
+section kstar
+
+open Computability
+
+lemma kstar_eq {α : Type*} (l : Language α) : l∗ = (l - 1)∗ := by
+  ext x
+  rw [Language.kstar_def_nonempty, Language.mem_kstar]
+  exact ⟨fun ⟨S, hx, h⟩ => ⟨S, ⟨hx, fun y ys => h y ys⟩⟩,
+    fun ⟨S, ⟨hx, h⟩⟩ => ⟨S, hx, fun y ys => h y ys⟩⟩
+
+lemma language_bddpath_kstar {n : ℕ} (flts : FLTS (Fin n) Symbol) (k : Fin n) :
+    language (BddPath.mk flts k k (k + 1)) = (language (BddPath.mk flts k k k))∗ := by
+  rw [← mul_one (language (BddPath.mk flts k k ↑k))∗]
+  rw [kstar_eq]
+  refine (Language.self_eq_mul_add_iff (by simp [Language.mem_sub])).mp ?_
+  -- mimic the proof of path2
+  ext xs
+  simp only [Language.mem_add, Language.mem_mul, Language.mem_sub]
+  constructor
+  · intro h
+    by_cases h' : xs ∈ (1 : Language Symbol)
+    · grind
+    left
+    use splitFirst flts k k xs, splitFirst_mem' h' h,
+      splitFirstCompl flts k k xs, splitFirstCompl_mem h,
+      splitFirst_append flts _ _ _
+  · rintro (⟨ys, ⟨⟨⟨hys, hsuppys⟩, hysnotempty⟩, ⟨zs, ⟨⟨hzs, hsuppzs⟩, happend⟩⟩⟩⟩ | hempty)
+    · refine ⟨by grind, ?_⟩
+      by_cases zs = []
+      · grind
+      rw [Language.mem_one] at hysnotempty
+      grind [pathSupp_append]
+    · rw [Language.mem_one] at hempty
+      simp only [mem_language, Accepts]
+      grind [PathSupp]
+
+end kstar
+
+open Computability
 /-
 Regex i j k is the regex for the path from state i to state j passing through states < k.
 When k = 0, i = j, the regex is ε union all characters from state i to state i.
@@ -354,5 +472,39 @@ noncomputable def Regex [Fintype Symbol] {n : ℕ} (flts : FLTS (Fin n) Symbol)
     else
       let kFin : Fin n := ⟨k, by omega⟩
       Regex flts i j k + Regex flts i kFin k * (Regex flts kFin kFin k).star * Regex flts kFin j k
+
+open RegularExpression
+
+variable {α : Type*}
+
+theorem mem_sum_matches'_iff (L : List (RegularExpression α)) (x : List α) :
+    x ∈ (L.sum).matches' ↔ ∃ P ∈ L, x ∈ P.matches' := by
+  induction L with
+  | nil => simp
+  | cons head tail ih =>
+  simp only [sum_cons, matches', Language.mem_add, ih, mem_cons, exists_eq_or_imp]
+
+theorem language_bddpath_eq_regex [Fintype Symbol] {n k : ℕ} {i j : Fin n}
+    {flts : FLTS (Fin n) Symbol} :
+    language (BddPath.mk flts i j k) = (Regex flts i j k).matches' := by
+  induction k generalizing i j with
+  | zero =>
+    ext xs
+    simp only [mem_language, Accepts, not_lt_zero, Regex]
+    rw [(by grind : (∀ i_1 ∈ PathSupp flts i xs, False) ↔ PathSupp flts i xs = ∅)]
+    split_ifs with heq
+    · -- The case of i = j, k = 0
+      simp only [matches', Language.mem_add, mem_sum_matches'_iff, pathSupp_empty_iff_empty_or_char]
+      aesop
+    · -- The case of i ≠ j, k = 0
+      rw [mem_sum_matches'_iff, pathSupp_empty_iff_empty_or_char]
+      aesop
+  | succ k ih =>
+    simp only [Regex]
+    split_ifs with hk
+    · rw [← ih, language_bddpath_eq_dfa flts i j hk, language_bddpath_eq_dfa flts i j (by omega)]
+    rw [language_bddpath_splitLast (k := ⟨k, by omega⟩), language_bddpath_splitFirst,
+      language_bddpath_kstar]
+    grind [matches'_add, matches'_mul, matches'_star]
 
 end Cslib.Language
